extraction/process_extraction.sh
@@ -1,0 +1,30 @@
+#!/usr/bin/env bash
+
+if [[ ! -f "plugin/src/concert_extraction_plugin.cmxs" ||
+      "plugin/src/concert_extraction_plugin.cmxs" -ot "theories/ExtractExtraction.vo" ]]
+then
+  cd plugin/src
+  # Uncapitalize modules to circumvent a bug of coqdep with mlpack files
+  for i in *.ml*
+  do
+    newi=`echo $i | cut -b 1 | tr '[:upper:]' '[:lower:]'``echo $i | cut -b 2-`;
+    if [[ ! $i -ef $newi ]]
+    then
+      echo "Moving " $i "to" $newi;
+      mv $i $newi;
+    fi
+  done
+
+  # This file was generated with
+  # cat template-coq/_PluginProject | grep "^[^#].*mli\?$" | sed "s/gen-src\///"
+  # from MetaCoq root
+  files=`cat ../template-coq-files.txt`
+  echo "Removing files linked in template-coq:" $files
+  rm -f $files
+
+  echo "Fixing extraction bugs"
+  sed -i "s/Coq__2/Coq__1/g" common1.mli
+  sed -i "s/Coq__3/Coq__1/g" common1.mli
+else
+  echo "Extraction up to date"
+fi
